File clean up

extraction/examples/RustEscrow.v
@@ -1,10 +1,18 @@
 From ConCert.Execution.Examples Require Import Escrow.
+From ConCert.Execution.Examples Require Import EscrowSolana.
 From ConCert.Extraction Require Import Common.
 From ConCert.Extraction Require Import ConcordiumExtract.
+From ConCert.Extraction Require Import SolanaExtract.
+From ConCert.Extraction Require Import RustExtract.
 From Coq Require Import Bool.
 From Coq Require Import String.
 From MetaCoq.Template Require Import All.
 
+
+Definition ESCROW_MODULE_SOLANA : SolanaMod _ :=
+  {| solana_contract_name := "Escrow";
+     solana_process := @ConCert.Execution.Examples.EscrowSolana.escrow_process;
+     solana_extra := []; |}.
 
 Definition ESCROW_MODULE : ConcordiumMod _ _ :=
   {| concmd_contract_name := "escrow"%string;
@@ -12,15 +20,36 @@ Definition ESCROW_MODULE : ConcordiumMod _ _ :=
      concmd_receive := @Escrow.receive;
      concmd_extra := []; |}.
 
-Definition should_inline kn :=
+(* Definition should_inline kn :=
   eq_kername kn <%% @Monads.bind %%>
   || eq_kername kn <%% Monads.Monad_option %%>
-  || if String.index 0 "setter_from_getter" (string_of_kername kn) then true else false.
+  || if String.index 0 "setter_from_getter" (string_of_kername kn) then true else false. *)
+
+Definition should_inline kn :=
+  eq_kername kn <%% @Monads.bind %%>
+  || eq_kername kn <%% @ProgramError.Monad_result_error %%>
+  || if String.index 0 "setter_from_getter" (string_of_kername kn) then true else false
+  || eq_kername <%% bool_rec %%> kn
+  || eq_kername <%% bool_rect %%> kn.
 
 (* NOTE: it is important to declare a priting config, otherwise MetaCoq evaluation tries to normalise a term with an unresolved instance and runs out of memory. *)
-Existing Instance DefaultPrintConfig.RustConfig.
+Instance RustConfig : RustPrintConfig :=
+    {| term_box_symbol := "()";
+       type_box_symbol := "()";
+       any_type_symbol := "()";
+       print_full_names := false |}.
 
-Redirect "/home/johnny/Documents/Tese/ConCert/extraction/examples/extracted-code/concordium-extract/escrow.rs"
+Redirect "/home/johnny/Documents/Tese/ConCert/extraction/examples/extracted-code/solana-extract/escrow.rs"
+MetaCoq Run (solana_extraction
+               ESCROW_MODULE_SOLANA
+               (SolanaRemap.build_remaps
+                  (SolanaRemap.remap_arith ++ SolanaRemap.remap_blockchain_consts ++ SolanaRemap.remap_aux_consts ++ SolanaRemap.remap_account_operations)
+                  []
+                  (SolanaRemap.remap_blockchain_inductives
+                     ++ SolanaRemap.remap_std_types))
+               should_inline).
+
+(* Redirect "/home/johnny/Documents/Tese/ConCert/extraction/examples/extracted-code/concordium-extract/escrow.rs"
 MetaCoq Run (concordium_extraction
                ESCROW_MODULE
                (ConcordiumRemap.build_remaps
@@ -29,4 +58,4 @@ MetaCoq Run (concordium_extraction
                   ConcordiumRemap.remap_inline_bool_ops
                   (ConcordiumRemap.remap_std_types
                      ++ ConcordiumRemap.remap_blockchain_inductives))
-               should_inline).
+               should_inline). *)
